Made all forall definitions opaque_to_smt in AlgebraTypes

AlgebraTypes.fst
@@ -7,8 +7,11 @@ type unary_op (a:Type) = a -> a
 type predicate (a:Type) = a -> bool
 type binary_relation (a: Type) = a -> a -> bool
 
+[@@"opaque_to_smt"]
 let is_reflexive  (#a:Type) (r: binary_relation a) = forall (x:a).     x `r` x
+[@@"opaque_to_smt"]
 let is_symmetric  (#a:Type) (r: binary_relation a) = forall (x y:a).   x `r` y == y `r` x
+[@@"opaque_to_smt"]
 let is_transitive (#a:Type) (r: binary_relation a) = forall (x y z:a). x `r` y /\ y `r` z ==> x `r` z 
 
 /// We do this for future work with fractions over arbitrary domains.
@@ -17,26 +20,30 @@ let is_transitive (#a:Type) (r: binary_relation a) = forall (x y z:a). x `r` y /
 /// (a/b)=(c/d) ==def== (ad=bc). The three properties shall be then proven explicitly.
 type equivalence_relation (a: Type) = r:binary_relation a{is_reflexive r /\ is_symmetric r /\ is_transitive r}
 
+[@@"opaque_to_smt"]
 let equivalence_wrt_condition (#a: Type) (op: binary_op a) (eq: equivalence_relation a) = 
   (forall (x y z:a). (x `eq` y) ==> ((x `op` z) `eq` (y `op` z))  /\ (z `op` x) `eq` (z `op` y))
   
 type equivalence_wrt (#a: Type) (op: binary_op a) = eq:equivalence_relation a{equivalence_wrt_condition op eq}
 
 let equivalence_is_symmetric (#a:Type) (eq: equivalence_relation a) (x:a) (y:a{x `eq` y})
-  : Lemma (x `eq` y == y `eq` x) = ()
+  : Lemma (x `eq` y == y `eq` x) = reveal_opaque (`%is_symmetric) (is_symmetric #a)
 
-private let eq_rel (a:Type) (eq: equivalence_relation a) : (t:equivalence_relation a {t == eq}) = eq
+//private let eq_rel (a:Type) (eq: equivalence_relation a) : (t:equivalence_relation a {t == eq}) = eq
 
 let trans_lemma (#a:Type) (eq: equivalence_relation a) (x y z:a)
-  : Lemma (requires ((x `eq` y) \/ (y `eq` x)) /\ ((y `eq` z) \/ (z `eq` y)))  (ensures x `eq` z && z `eq` x) = ()
-
+  : Lemma (requires ((x `eq` y) \/ (y `eq` x)) /\ ((y `eq` z) \/ (z `eq` y)))  (ensures x `eq` z && z `eq` x)   
+  = reveal_opaque (`%is_transitive) (is_transitive #a);
+    reveal_opaque (`%is_symmetric) (is_symmetric #a)
 
 private let trans_lemma_4 (#a:Type) (eq: equivalence_relation a) (x:a)
                                                                  (y:a{eq x y \/ eq y x})
                                                                  (z:a{eq y z \/ eq z y})
-                                                                 (w:a{eq z w \/ eq w z}) : Lemma (x `eq` w /\ w `eq` x) = ()
+                                                                 (w:a{eq z w \/ eq w z})
+  : Lemma (x `eq` w /\ w `eq` x) = reveal_opaque (`%is_transitive) (is_transitive #a);
+                                  reveal_opaque (`%is_symmetric) (is_symmetric #a)
 
-let symm_lemma (#a:Type) (eq:equivalence_relation a) (x:a) (y:a) : Lemma (x `eq` y == y `eq` x) = ()
+let symm_lemma (#a:Type) (eq:equivalence_relation a) (x:a) (y:a) : Lemma (x `eq` y == y `eq` x) = reveal_opaque (`%is_symmetric) (is_symmetric #a) 
 
 /// FStar does not automatically apply lemmas on equivalence being symmetric reflexive and transitive.
 /// So, I at least make my lemmas such that I care about `eq` operand order as little as possible
@@ -47,7 +54,8 @@ let equivalence_wrt_operation_lemma (#a: Type) (#op: binary_op a) (eq: equivalen
     (e1 `op` z) `eq` (e2 `op` z) /\    
     (e2 `op` z) `eq` (e1 `op` z) /\    
     (z `op` e1) `eq` (z `op` e2) /\
-    (z `op` e2) `eq` (z `op` e1)) = ()
+    (z `op` e2) `eq` (z `op` e1)) = reveal_opaque (`%equivalence_wrt_condition) (equivalence_wrt_condition #a);
+                                    reveal_opaque (`%is_symmetric) (is_symmetric #a) 
     
 let eq_wrt_emulated (#a:Type) (#op: binary_op a) (eq: equivalence_relation a{equivalence_wrt_condition op eq}) (e1 e2 z: a)
   : Lemma 
@@ -63,48 +71,73 @@ let eq_wrt_emulated (#a:Type) (#op: binary_op a) (eq: equivalence_relation a{equ
 ///
 /// The forall part has precisely the meaning we expect it to have :)
 /// From here, one can deduce what an exists statement would look like...
+[@@"opaque_to_smt"]
 let is_associative (#a:Type) (op:binary_op a) (eq: equivalence_relation a) = forall (x y z:a). ((x `op` y) `op` z) `eq` (x `op` (y `op` z))
+[@@"opaque_to_smt"]
 let is_commutative (#a:Type) (op:binary_op a) (eq: equivalence_relation a) = forall (x y:a). (x `op` y) `eq` (y `op` x)
 
+
 let associative_operation_lemma (#a:Type) (eq: equivalence_relation a) (op:binary_op a{is_associative op eq}) (x y z:a) 
-  : Lemma (
-            ((x `op` y) `op` z) `eq` (x `op` (y `op` z)) && (x `op` (y `op` z)) `eq` ((x `op` y) `op` z)
-          )
-  = ()
+  : Lemma (((x `op` y) `op` z) `eq` (x `op` (y `op` z)) && (x `op` (y `op` z)) `eq` ((x `op` y) `op` z))
+  = reveal_opaque (`%is_associative) (is_associative #a);
+    reveal_opaque (`%is_symmetric) (is_symmetric #a) 
+  
 
 let commutative_substitution_lemma (#a:Type) (#eq: equivalence_relation a) (op: binary_op a{is_commutative op eq}) 
-  (x y z: a) : Lemma (x `eq` (y `op` z) == x `eq` (z `op` y)) = ()
+  (x y z: a) : Lemma (x `eq` (y `op` z) == x `eq` (z `op` y)) = 
+  reveal_opaque (`%is_commutative) (is_commutative #a);
+  reveal_opaque (`%is_transitive) (is_transitive #a) 
 
 let associative_lemma_for_substitution (#a:Type) (eq: equivalence_relation a)
   (op: binary_op a{is_associative op eq}) (x y z w: a)
-  : Lemma ( ((x `op` y) `op` z) `eq` w == (x `op` (y `op` z)) `eq` w) = ()
-
+  : Lemma ( ((x `op` y) `op` z) `eq` w == (x `op` (y `op` z)) `eq` w) = 
+  reveal_opaque (`%is_associative) (is_associative #a);
+  reveal_opaque (`%is_transitive) (is_transitive #a); 
+  reveal_opaque (`%is_symmetric) (is_symmetric #a) 
+  
+[@@"opaque_to_smt"]
 let is_idempotent (#a:Type) (r: unary_op a) (eq: equivalence_relation a)  = forall (x:a). (r x) `eq` (r (r x))
 
 /// Things quickly get funny if we consider non-associative structures (magmas etc).
 /// Therefore we don't, not because we dislike fun, but because we strive for sanity.
 
+
+[@@"opaque_to_smt"]
 let is_left_id_of  (#a:Type) (u:a) (op:binary_op a) (eq: equivalence_relation a) = forall (x:a). (u `op` x) `eq` x // left identity
+[@@"opaque_to_smt"]
 let is_right_id_of (#a:Type) (u:a) (op:binary_op a) (eq: equivalence_relation a) = forall (x:a). (x `op` u) `eq` x // right identity
+[@@"opaque_to_smt"]
 let is_neutral_of  (#a:Type) (u:a) (op:binary_op a) (eq: equivalence_relation a) = is_left_id_of u op eq /\ is_right_id_of u op eq // neutral element
-let is_inverse_element_of (#a: Type) (op: binary_op a) (eq: equivalence_relation a) (neutral: a) (x: a) (y: a) 
-  = ((x `op` y) `eq` neutral) /\ ((y `op` x) `eq` neutral)
-let is_invertible_element_of (#a: Type) (op: binary_op a) (eq: equivalence_relation a) (neutral: a) (x: a) 
-  = exists (y: a). (is_inverse_element_of op eq neutral x y)
+
 type neutral_element_of (#a: Type) (op: binary_op a) (eq: equivalence_relation a) = (x:a{is_neutral_of x op eq})
 
 let neutral_lemma (#a:Type) (op: binary_op a) (eq: equivalence_relation a) (x: neutral_element_of op eq) (y:a)
-  : Lemma ((x `op` y) `eq` y /\ (y `op` x) `eq` y) = ()
-
-
+  : Lemma ((x `op` y) `eq` y /\ (y `op` x) `eq` y) = 
+  reveal_opaque (`%is_left_id_of) (is_left_id_of #a); 
+  reveal_opaque (`%is_right_id_of) (is_right_id_of #a); 
+  reveal_opaque (`%is_neutral_of) (is_neutral_of #a)
+  
 /// If you see something trivial, then it is either here to reduce the rlimit for some bigger lemma,
 /// or a leftover from time where something didn't verify and I made more and more explicit lemmas,
 /// or it should be deleted. I periodically cleanup this file and remove unused lemmas.
 /// Nothing big gets removed anyway.
 
-let neutral_is_unique (#a:Type) (op: binary_op a) (eq: equivalence_wrt op) (u: neutral_element_of op eq) (v: neutral_element_of op eq) : Lemma (eq u v) = ()
+let neutral_is_unique (#a:Type) (op: binary_op a) (eq: equivalence_wrt op) (u: neutral_element_of op eq) (v: neutral_element_of op eq) 
+  : Lemma (eq u v) = 
+  reveal_opaque (`%is_transitive) (is_transitive #a); 
+  reveal_opaque (`%is_symmetric) (is_symmetric #a);  
+  reveal_opaque (`%is_left_id_of) (is_left_id_of #a); 
+  reveal_opaque (`%is_right_id_of) (is_right_id_of #a);
+  reveal_opaque (`%is_neutral_of) (is_neutral_of #a)
+  
 
-let neutral_equivalent_is_neutral (#a:Type) (op: binary_op a) (eq: equivalence_wrt op) (x: neutral_element_of op eq) (y: a{y `eq` x}) : Lemma (is_neutral_of y op eq) =   
+let neutral_equivalent_is_neutral (#a:Type) (op: binary_op a) (eq: equivalence_wrt op) (x: neutral_element_of op eq) (y: a{y `eq` x}) : Lemma (is_neutral_of y op eq) =    
+  reveal_opaque (`%is_transitive) (is_transitive #a); 
+  reveal_opaque (`%is_symmetric) (is_symmetric #a); 
+  reveal_opaque (`%is_left_id_of) (is_left_id_of #a); 
+  reveal_opaque (`%is_right_id_of) (is_right_id_of #a);
+  reveal_opaque (`%is_neutral_of) (is_neutral_of #a);
+  reveal_opaque (`%equivalence_wrt_condition) (equivalence_wrt_condition #a); 
   let aux (t:a) : Lemma (((t `op` y) `eq` t) /\ ((y `op` t) `eq` t)) = equivalence_wrt_operation_lemma eq x y t in
   FStar.Classical.forall_intro aux;
   assert (is_neutral_of y op eq);
@@ -113,26 +146,47 @@ let neutral_equivalent_is_neutral (#a:Type) (op: binary_op a) (eq: equivalence_w
 
 /// The notion of absorbing element, or absorber, is the generalization of integer zero with respect to multiplication
 /// That is, 0x = x0 = 0. Other exmaples are the empty set w.r.t. intersection, 1 w.r.t. GCD in naturals, etc.
+[@@"opaque_to_smt"]
 let is_absorber_of (#a:Type) (z:a) (op:binary_op a) (eq: equivalence_relation a) = forall (x:a). ((x `op` z) `eq` z) && ((z `op` x) `eq` z)
-type absorber_of (#a:Type) (op:binary_op a) (eq: equivalence_relation a) = z:a{is_absorber_of z op eq}
-type non_absorber_of (#a:Type) (op: binary_op a) (eq: equivalence_relation a) = z:a{~(is_absorber_of z op eq)}
+
+unfold type absorber_of (#a:Type) (op:binary_op a) (eq: equivalence_relation a) = z:a{is_absorber_of z op eq}
+unfold type non_absorber_of (#a:Type) (op: binary_op a) (eq: equivalence_relation a) = z:a{~(is_absorber_of z op eq)}
 
 let absorber_lemma (#a:Type) (op:binary_op a) (eq: equivalence_relation a) (z: a{is_absorber_of z op eq}) (x:a)
-  : Lemma ((z `op` x) `eq` z /\ (x `op` z) `eq` z) = ()
+  : Lemma ((z `op` x) `eq` z /\ (x `op` z) `eq` z) = 
+  reveal_opaque (`%is_absorber_of) (is_absorber_of #a)
 
 /// Proving that in any magma, there may not be 2 distinct absorbers, is left as an exercise to both Z3 and the reader.
 /// And Z3 is doing fine on that account, just saying.
-let absorber_is_unique (#a:Type) (op: binary_op a) (eq: equivalence_relation a) (z1 z2: a) : Lemma (requires is_absorber_of z1 op eq /\ is_absorber_of z2 op eq) (ensures eq z1 z2 /\ eq z2 z1) = ()
+let absorber_is_unique (#a:Type) (op: binary_op a) (eq: equivalence_relation a) (z1 z2: a) 
+  : Lemma (requires is_absorber_of z1 op eq /\ is_absorber_of z2 op eq) 
+          (ensures eq z1 z2 /\ eq z2 z1) = 
+  reveal_opaque (`%is_transitive) (is_transitive #a); 
+  reveal_opaque (`%is_symmetric) (is_symmetric #a); 
+  reveal_opaque (`%is_absorber_of) (is_absorber_of #a)
+  
 
-let absorber_eq_is_abs (#a:Type) (op: binary_op a) (eq: equivalence_wrt op) (z1: absorber_of op eq) (z2: a{z2 `eq` z1}) (t: a) : Lemma (t `op` z2 `eq` z2 /\ z2 `op` t `eq` z2) = equivalence_wrt_operation_lemma eq z1 z2 t 
+let absorber_eq_is_abs (#a:Type) (op: binary_op a) (eq: equivalence_wrt op) (z1: absorber_of op eq) (z2: a{z2 `eq` z1}) (t: a) 
+  : Lemma (t `op` z2 `eq` z2 /\ z2 `op` t `eq` z2) =   
+  reveal_opaque (`%is_transitive) (is_transitive #a); 
+  reveal_opaque (`%is_symmetric) (is_symmetric #a); 
+  reveal_opaque (`%is_absorber_of) (is_absorber_of #a);
+  equivalence_wrt_operation_lemma eq z1 z2 t 
 
-let absorber_equal_is_absorber (#a:Type) (op:binary_op a) (eq: equivalence_wrt op) (z1: absorber_of op eq) (z2:a{z2 `eq` z1}) : Lemma (is_absorber_of z2 op eq) = 
+let absorber_equal_is_absorber (#a:Type) (op:binary_op a) (eq: equivalence_wrt op) (z1: absorber_of op eq) (z2:a{z2 `eq` z1}) 
+  : Lemma (is_absorber_of z2 op eq) = 
+  reveal_opaque (`%is_absorber_of) (is_absorber_of #a);
   FStar.Classical.forall_intro (absorber_eq_is_abs op eq z1 z2)
 
 let absorber_equal_is_absorber_req (#a:Type) (op: binary_op a) (eq: equivalence_wrt op) (z1 z2: a) 
-  : Lemma (requires is_absorber_of z1 op eq /\ eq z1 z2) (ensures is_absorber_of z2 op eq) = absorber_equal_is_absorber op eq z1 z2
+  : Lemma (requires is_absorber_of z1 op eq /\ eq z1 z2) 
+          (ensures is_absorber_of z2 op eq) = 
+  reveal_opaque (`%is_absorber_of) (is_absorber_of #a); 
+  reveal_opaque (`%is_symmetric) (is_symmetric #a);           
+  absorber_equal_is_absorber op eq z1 z2
   
-let nonabsorber_equal_is_nonabsorber (#a:Type) (op: binary_op a) (eq: equivalence_wrt op) (p: non_absorber_of op eq) (q:a{q `eq` p}) : Lemma (~(is_absorber_of q op eq)) 
+let nonabsorber_equal_is_nonabsorber (#a:Type) (op: binary_op a) (eq: equivalence_wrt op) (p: non_absorber_of op eq) (q:a{q `eq` p}) 
+  : Lemma (~(is_absorber_of q op eq)) 
   = (Classical.move_requires (absorber_equal_is_absorber_req op eq q)) p
 
 
@@ -143,11 +197,13 @@ let nonabsorber_equal_is_nonabsorber (#a:Type) (op: binary_op a) (eq: equivalenc
 ///
 /// For arbitrary domains, there is no hope of reduced fractions, so the notions for inverses and neutrals
 /// stays in its most general form.
+[@@"opaque_to_smt"]
 let is_inverse_operation_for (#a: Type) (inv: unary_op a) (op: binary_op a) (eq: equivalence_relation a) 
   = (forall (x:a). is_neutral_of (op x (inv x)) op eq /\ is_neutral_of (op (inv x) x) op eq)
 
 let inverse_operation_lemma (#a:Type) (op: binary_op a) (eq: equivalence_wrt op) (inv: unary_op a{is_inverse_operation_for inv op eq}) (x: a) 
-  : Lemma (is_neutral_of (x `op` (inv x)) op eq /\ is_neutral_of ((inv x) `op` x) op eq) = ()
+  : Lemma (is_neutral_of (x `op` (inv x)) op eq /\ is_neutral_of ((inv x) `op` x) op eq) = 
+  reveal_opaque (`%is_inverse_operation_for) (is_inverse_operation_for #a)
 
 /// The inverse operation type is also a refinement for arbitrary unary operation 
 type inverse_op_for (#a: Type) (op: binary_op a) (eq: equivalence_relation a) 
@@ -156,55 +212,62 @@ type inverse_op_for (#a: Type) (op: binary_op a) (eq: equivalence_relation a)
 let inverses_produce_neutral (#a:Type) (eq: equivalence_relation a) (op: binary_op a{is_associative op eq /\ equivalence_wrt_condition op eq}) (inv: inverse_op_for op eq) (x y: a)
   : Lemma (requires inv x `eq` y)
           (ensures is_neutral_of (x `op` y) op eq) =
-   // assert_spinoff ((inv x `eq` y));
- //   assert (is_neutral_of (x `op` inv x) op eq);
     equivalence_wrt_operation_lemma #a #op eq (inv x) y x;
-  //  assert (x `op` y `eq` (x `op` inv x));
+    reveal_opaque (`%is_inverse_operation_for) (is_inverse_operation_for #a);
     neutral_equivalent_is_neutral op eq (x `op` inv x) (x `op` y)
 
 let group_operation_lemma (#a:Type) (eq: equivalence_relation a) 
                              (op: binary_op a{is_associative op eq /\ equivalence_wrt_condition op eq}) 
                              (inv: inverse_op_for op eq) (x y z:a) 
-  : Lemma (requires (x `op` z) `eq` (y `op` z)) (ensures (x `eq` y)) = 
+  : Lemma (requires (x `op` z) `eq` (y `op` z)) (ensures (x `eq` y)) =    
+  reveal_opaque (`%is_transitive) (is_transitive #a); // we're going to need the transitivity of ==
+  let eq_wrt_lemma = equivalence_wrt_operation_lemma #a #op eq in
   let z'  = inv z in
   let op = op in
-  let eq : equivalence_wrt op = eq in
+  let eq  = eq in
   let zz' = z `op` z' in
-  let xz = x `op` z in                         // suppose zz'    = 0 (always possible in a group)
+  let xz = x `op` z in                         // suppose zz'    = 1 (always possible in a group)
   let yz = y `op` z in                         // we have xz     = yz
-  equivalence_wrt_operation_lemma eq xz yz z'; // then,   (xz)z' = (yz)z'
+  eq_wrt_lemma xz yz z';                       // then,   (xz)z' = (yz)z'
   associative_operation_lemma eq op x z z';    // or,     x(zz') = (yz)z'
-  neutral_lemma op eq zz' x;                   // zz'=0,   (zz') = x
+  inverse_operation_lemma op eq inv z;         // as we know, zz'= 1
+  neutral_lemma op eq zz' x;                   // zz'=1,  (zz')x = x
   trans_lemma eq (xz `op` z') (x `op` zz') x;  // transitivity, (xz)z' = x(zz') = x, (xz)z'=x
   trans_lemma eq x (xz `op` z') (yz `op` z');  // transitivity, x = (xz)z' = (yz)z'
   associative_operation_lemma eq op y z z';    // assoc again, (yz)z' = y(zz') 
   neutral_lemma op eq zz' y;                   // neutral again, y(zz')=y.
   ()                                           // the rest is left as an exercise for Z3
 
- 
-#push-options "--ifuel 0 --fuel 0 --z3rlimit 2"
-let producing_neutral_means_inverses (#a:Type) (eq: equivalence_relation a) (op: binary_op a{is_associative op eq /\ equivalence_wrt_condition op eq}) (inv: inverse_op_for op eq) (x y: a)
-  : Lemma (requires is_neutral_of (x `op` y) op eq) (ensures inv x `eq` y)  = 
   
+let producing_neutral_means_inverses (#a:Type) 
+                                     (eq: equivalence_relation a) 
+                                     (op: binary_op a{is_associative op eq /\ equivalence_wrt_condition op eq}) 
+                                     (inv: inverse_op_for op eq) 
+                                     (x y: a)
+  : Lemma (requires is_neutral_of (x `op` y) op eq) 
+          (ensures inv x `eq` y) = 
+  reveal_opaque (`%is_neutral_of) (is_neutral_of #a); 
+  reveal_opaque (`%is_transitive) (is_transitive #a); 
+  inverse_operation_lemma op eq inv y;
+  inverse_operation_lemma op eq inv x;
   assert (is_neutral_of (inv y `op` y) op eq);
-//  assert (is_neutral_of (x `op` y) op eq);
+  // assert (is_neutral_of (x `op` y) op eq);
   neutral_is_unique op eq  (inv y `op` y) (x `op` y);
   group_operation_lemma eq op inv (inv y) x y;
-//  assert (inv y `eq` x);
+  // assert (inv y `eq` x);
   equivalence_wrt_operation_lemma #a #op eq (inv y) x y;
   equivalence_wrt_operation_lemma #a #op eq (y `op` inv y) (y `op` x) (inv x);  
-//  assert (((y `op` inv y) `op` inv x) `eq` ((y `op` x) `op` (inv x)));
-//  assert (is_neutral_of (y `op` inv y) op eq);
+  // assert (((y `op` inv y) `op` inv x) `eq` ((y `op` x) `op` (inv x)));
+  // assert (is_neutral_of (y `op` inv y) op eq);
   neutral_lemma op eq (y `op` inv y) (inv x);
-//  assert ((inv x) `eq` ((y `op` x) `op` (inv x)));
+  // assert ((inv x) `eq` ((y `op` x) `op` (inv x)));
   associative_operation_lemma eq op y x (inv x);
-//  assert ((inv x) `eq` (y `op` (x `op` inv x)));
+  // assert ((inv x) `eq` (y `op` (x `op` inv x)));
   neutral_lemma op eq (x `op` inv x) y;
   trans_lemma eq (inv x) (y `op` (x `op` inv x)) y;
-//  assert (inv x `eq` y);
-//  assert_spinoff (inv x `eq` y == true);
-  ()
-#pop-options
+  // assert (inv x `eq` y);
+  // assert_spinoff (inv x `eq` y == true);
+  () 
 
 let equivalence_lemma_from_implications (#a:Type) (p) (q)
                                         (to_right : (x:a)->(y:a)->Lemma (requires p x y) (ensures q x y))
@@ -213,48 +276,47 @@ let equivalence_lemma_from_implications (#a:Type) (p) (q)
                                         : Lemma (p x y <==> q x y) = 
                                         (Classical.move_requires_2 to_right) x y;
                                         (Classical.move_requires_2 to_left) x y
- 
-(*
-let inverses_produce_neutral (#a:Type) (eq: equivalence_relation a) (op: binary_op a{is_associative op eq /\ equivalence_wrt_condition op eq}) (inv: inverse_op_for op eq) (x y: a)
-  : Lemma (requires (inv x `eq` y))
-          (ensures is_neutral_of (x `op` y) op eq) =
-*)
-
-#push-options "--ifuel 0 --fuel 0 --z3rlimit 14"
-  let inverse_lemma_def (#a:Type) (eq: equivalence_relation a) (op: binary_op a{is_associative op eq /\ equivalence_wrt_condition op eq}) (inv: inverse_op_for op eq) (x y: a)
+   
+let inverse_lemma_def (#a:Type) (eq: equivalence_relation a) (op: binary_op a{is_associative op eq /\ equivalence_wrt_condition op eq}) (inv: inverse_op_for op eq) (x y: a)
   : Lemma (is_neutral_of (x `op` y) op eq <==> inv x `eq` y) = 
   (FStar.Classical.move_requires_2 (inverses_produce_neutral eq op inv)) x y;
   (FStar.Classical.move_requires_2 (producing_neutral_means_inverses eq op inv)) x y;
   assert (is_neutral_of (op x y) op eq ==> inv x `eq` y);   
-  () 
-#pop-options
-
- 
+  ()  
 
 /// We shall generally keep in mind that distributivity laws must be considered separately
 /// If in future we consider K[x] with multiplication f(x)*g(x) defined as composition f(g(x)),
 /// we will do well to remember that only one of the two distributivities holds there.
+[@@"opaque_to_smt"]
 let is_left_distributive (#a:Type) (op_mul:binary_op a) (op_add:binary_op a) (eq: equivalence_relation a) =
   forall (x y z:a). (x `op_mul` (y `op_add` z)) `eq` ((x `op_mul` y) `op_add` (x `op_mul` z))
+[@@"opaque_to_smt"]
 let is_right_distributive (#a:Type) (op_mul:binary_op a) (op_add:binary_op a) (eq: equivalence_relation a) =
   forall (x y z:a). ((x `op_add` y) `op_mul` z) `eq` ((x `op_mul` z) `op_add` (y `op_mul` z))
+[@@"opaque_to_smt"]
 let is_fully_distributive (#a:Type) (op_mul:binary_op a) (op_add:binary_op a) (eq: equivalence_relation a) =
   forall (x y z:a). ((x `op_mul` (y `op_add` z)) `eq` ((x `op_mul` y) `op_add` (x `op_mul` z))) /\ (((x `op_add` y) `op_mul` z) `eq` ((x `op_mul` z) `op_add` (y `op_mul` z)))
 
 let fully_distributive_is_both_left_and_right  (#a:Type) (op_mul:binary_op a) (op_add:binary_op a) (eq: equivalence_relation a) 
   : Lemma (is_fully_distributive op_mul op_add eq <==> is_left_distributive op_mul op_add eq /\ is_right_distributive op_mul op_add eq)  
-  = ()
+  = reveal_opaque (`%is_left_distributive) (is_left_distributive #a);  
+    reveal_opaque (`%is_right_distributive) (is_right_distributive #a);
+    reveal_opaque (`%is_fully_distributive) (is_fully_distributive #a)
 
 let left_distributivity_lemma (#a:Type) (op_mul:binary_op a) (op_add:binary_op a) (eq: equivalence_relation a) (x y z: a)
-  : Lemma (requires is_left_distributive op_mul op_add eq) (ensures (x `op_mul` (y `op_add` z)) `eq` ((x `op_mul` y) `op_add` (x `op_mul` z))) = ()
+  : Lemma (requires is_left_distributive op_mul op_add eq) (ensures (x `op_mul` (y `op_add` z)) `eq` ((x `op_mul` y) `op_add` (x `op_mul` z))) 
+  = reveal_opaque (`%is_left_distributive) (is_left_distributive #a)
 
 let right_distributivity_lemma (#a:Type) (op_mul:binary_op a) (op_add:binary_op a) (eq: equivalence_relation a) (x y z: a)
-  : Lemma (requires is_right_distributive op_mul op_add eq) (ensures ((x `op_add` y) `op_mul` z) `eq` ((x `op_mul` z) `op_add` (y `op_mul` z))) = ()
+  : Lemma (requires is_right_distributive op_mul op_add eq) (ensures ((x `op_add` y) `op_mul` z) `eq` ((x `op_mul` z) `op_add` (y `op_mul` z))) 
+  = reveal_opaque (`%is_right_distributive) (is_right_distributive #a) 
 
 /// Domain defining property (the alternative form is the Cancellation Law, (ax=bx ==> (x=0 \/ a=b)
-let has_no_zero_divisors (#a:Type) (zero:a) (op_mul: binary_op a) (eq: equivalence_relation a)=
+[@@"opaque_to_smt"]
+let has_no_zero_divisors (#a:Type) (zero:a) (op_mul: binary_op a) (eq: equivalence_relation a) =
   forall (x y:a). ((x `op_mul` y) `eq` zero) ==> (x `eq` zero) \/ (y `eq` zero)
 /// For future reference, we difine what it means for divisor to divide dividend
+[@@"opaque_to_smt"]
 let is_divisor_of (#a:Type) (op_mul: binary_op a) (eq: equivalence_relation a) (divisor: a) (dividend: a) = 
   exists (quotient: a). (quotient `op_mul` divisor) `eq` dividend
 
@@ -262,10 +324,13 @@ let is_divisor_of (#a:Type) (op_mul: binary_op a) (eq: equivalence_relation a) (
 /// We provide the two lemmas that ensure divides, second one purely to
 /// demonstrate how one uses exists_intro. Usually you're fine with '= ()'.
 let inst_divides (#a:Type) (op_mul: binary_op a) (eq: equivalence_relation a) (y: a) (x: a) (z:a{(z `op_mul` y) `eq` x})
-  : Lemma (is_divisor_of op_mul eq y x) = ()
+  : Lemma (is_divisor_of op_mul eq y x) = reveal_opaque (`%is_divisor_of) (is_divisor_of #a) 
+  
 /// explicitly stated version showcases FStar.Classical.exists_intro
 let inst_divides_2 (#a:Type) (op_mul: binary_op a) (eq: equivalence_relation a) (y: a) (x: a) (z:a{(z `op_mul` y) `eq` x})
-  : Lemma (is_divisor_of op_mul eq y x) = FStar.Classical.exists_intro (fun z -> (z `op_mul` y) `eq` x) z
+  : Lemma (is_divisor_of op_mul eq y x) = 
+  reveal_opaque (`%is_divisor_of) (is_divisor_of #a);
+  FStar.Classical.exists_intro (fun z -> (z `op_mul` y) `eq` x) z
 
 /// This will soon be used as we'll represent elements in form of x=(unit_part)*(normal_part)
 /// where (unit_part) is a ring unit, and (normal_part) is, roughly speaking, (unit_part⁻¹ * x),
@@ -276,27 +341,27 @@ let inst_divides_2 (#a:Type) (op_mul: binary_op a) (eq: equivalence_relation a) 
 ///
 /// we denote the unit u, because the word `unit` is reserved in F*
 /// Invertible elements in a ring are called units, and here's their defining condition
+[@@"opaque_to_smt"]
 let is_unit (#a: Type) (x: a) (op:binary_op a) (eq: equivalence_relation a) 
   = exists (y:a). (is_neutral_of (x `op` y) op eq /\ is_neutral_of (y `op` x) op eq)
-/// A zero of a ring is the neutral element of the ring's additive group,
-/// and here's the special property we might need in the future
-let is_zero (#a: Type) (z: a) (op_mul: binary_op a) (eq: equivalence_relation a) = forall (x: a). ((x `op_mul` z) `eq` z) /\ ((z `op_mul` x) `eq` z)
+  
 /// We call the two elements associated if they divide each other
 let are_associated (#a: Type) (p: a) (q: a) (op_mul: binary_op a) (eq: equivalence_relation a) = (is_divisor_of op_mul eq p q) /\ (is_divisor_of op_mul eq q p) 
 
 /// We also define in advance the notions of irreducibles and primes
 /// We don't tell one from the other in Z, but in general, they are not the same thing.
+[@@"opaque_to_smt"]
 let is_irreducible (#a: Type) (x: a) (op_mul: binary_op a) (eq: equivalence_relation a) = 
   (~(is_unit x op_mul eq)) /\
   (exists (neutral: a). is_neutral_of neutral op_mul eq) /\  
   (forall (p q: a). ((q `op_mul` p) `eq` x) ==> ( (are_associated p x op_mul eq) /\ (is_unit q op_mul eq)) 
                                       \/ ((are_associated q x op_mul eq) /\ (is_unit p op_mul eq)))
-                                      
+[@@"opaque_to_smt"]                                     
 let is_prime (#a: Type) (p: a) (one: a) (op_mul: binary_op a) (eq: equivalence_relation a) = 
   (~(is_unit p op_mul eq)) /\ (forall (m n: a). (is_divisor_of op_mul eq p (m `op_mul` n)) ==> ((is_divisor_of op_mul eq p m) \/ (is_divisor_of op_mul eq p n)))
 
-let respects_equivalence (#a:Type) (f: unary_op a) (eq: equivalence_relation a) = 
-  forall (x y:a). (x `eq` y) ==> (f x) `eq` (f y)
+[@@"opaque_to_smt"]  
+let respects_equivalence (#a:Type) (f: unary_op a) (eq: equivalence_relation a) = forall (x y:a). (x `eq` y) ==> (f x) `eq` (f y)
 
 noeq type magma (#a: Type) = 
 {
@@ -316,75 +381,68 @@ type commutative_group (#a:Type)     = g: group #a{is_commutative g.op g.eq}
 
 let magma_eq_wrt_condition (#a:Type) (m: magma #a) : Lemma(equivalence_wrt_condition m.op m.eq) = ()
 
-
 let absorber_never_equals_non_absorber (#a: Type) (op: binary_op a) (eq: equivalence_wrt op) 
   (x: absorber_of op eq) (y: non_absorber_of op eq) : Lemma (~(x `eq` y)) = 
+  reveal_opaque (`%is_symmetric) (is_symmetric #a);   
   if (x `eq` y) then absorber_equal_is_absorber op eq x y
 
-let plus_associative 
-  (#a:Type) 
-  (op: binary_op a) 
-  (eq: equivalence_wrt op)  
-  (x y z: a)
-  : Lemma
-  (requires is_associative op eq)
-  (ensures  ((x `op` y) `op` z) `eq` (x `op` (y `op` z))) = ()
-
-let is_absorber_of_magma (#a:Type) (z: a) (m: magma #a) = is_absorber_of z m.op m.eq
+unfold let is_absorber_of_magma (#a:Type) (z: a) (m: magma #a) = is_absorber_of z m.op m.eq
 
 /// When I try to keep the rlimit at minimum, lemmas like this one sometimes help
 let neutral_inverse_is_neutral (#a:Type) (g: group #a) : Lemma (g.neutral `g.eq` (g.inv g.neutral)) =  
-  assert ((g.neutral `g.op` (g.inv g.neutral)) `g.eq` g.neutral)
+  reveal_opaque (`%is_symmetric) (is_symmetric #a);   
+  reveal_opaque (`%is_transitive) (is_transitive #a);
+  neutral_lemma g.op g.eq g.neutral (g.inv g.neutral);
+  inverse_operation_lemma g.op g.eq g.inv g.neutral;
+  neutral_is_unique g.op g.eq g.neutral (g.neutral `g.op` g.inv g.neutral)
 
 let group_op_lemma (#a:Type) (g: group #a) (x y z:a) 
-  : Lemma (requires (x `g.op` z) `g.eq` (y `g.op` z)) (ensures (x `g.eq` y)) = group_operation_lemma g.eq g.op g.inv x y z
+  : Lemma (requires (x `g.op` z) `g.eq` (y `g.op` z)) (ensures (x `g.eq` y)) 
+  = group_operation_lemma g.eq g.op g.inv x y z
 
 
 #push-options "--ifuel 1 --fuel 0 --z3rlimit 16"
-let group_element_equality_means_zero_difference (#a:Type) (g: group #a) (x y: a) : Lemma (x `g.eq` y <==> (x `g.op` g.inv y) `g.eq` g.neutral) = 
-  inverse_operation_lemma g.op g.eq g.inv y; //isneutral(y + -y), x + -y
-  neutral_is_unique g.op g.eq  (g.op y (g.inv y)) g.neutral; 
-  assert ((g.op y (g.inv y)) `g.eq` g.neutral);
+let group_element_equality_means_zero_difference (#a:Type) (g: group #a) (x y: a) 
+  : Lemma (x `g.eq` y <==> (x `g.op` g.inv y) `g.eq` g.neutral) = 
+  inverse_operation_lemma g.op g.eq g.inv y;                   // is_neutral (y + -y), x + -y
+  neutral_is_unique g.op g.eq  (g.op y (g.inv y)) g.neutral;   // (y + (-y) = 0
   if (x `g.eq` y) then (
     equivalence_wrt_operation_lemma g.eq x y (g.inv y);
     assert ((x `g.op` g.inv y) `g.eq` (y `g.op` g.inv y));
-    trans_lemma g.eq (x `g.op` g.inv y) (y `g.op` g.inv y) g.neutral;
-    ()    
+    trans_lemma g.eq (x `g.op` g.inv y) (y `g.op` g.inv y) g.neutral
   ) else (
     if ((x `g.op` g.inv y) `g.eq` g.neutral) then ( 
       trans_lemma g.eq (x `g.op` g.inv y) g.neutral (y `g.op` g.inv y);
-      group_op_lemma  g x y (g.inv y);
-      ()
+      group_op_lemma  g x y (g.inv y)
     ) 
-    else ( 
-      ()
-    )
   )
 
-let flip_lemma p1 p2 (q:unit -> Lemma (requires p1) (ensures p2))
-  : Lemma (requires ~p2) (ensures ~p1)
-  = FStar.Classical.move_requires q ()
-
-#push-options "--ifuel 0 --fuel 0 --z3rlimit 4 --query_stats"
 let absorber_for_invertible_operation_is_nonsense (#a:Type) (op: binary_op a) (eq: equivalence_wrt op) (inv: inverse_op_for op eq)
-   (y: non_absorber_of op eq) (z:a) : Lemma (requires is_absorber_of z op eq) (ensures False) =  
+   (y: non_absorber_of op eq) (z:a) : Lemma (requires is_absorber_of z op eq) (ensures False) =   
+    reveal_opaque (`%is_absorber_of) (is_absorber_of #a);  
     absorber_never_equals_non_absorber op eq z y;
     let z' = inv z in
-    let zz' = op z (inv z) in
+    let zz' = op z z' in
+    absorber_lemma op eq z z';
+    inverse_operation_lemma op eq inv z;                  // zz' is the neutral element
     let yzz' = op y zz' in                                // I write "the absorber" here to underline its uniqueness
     absorber_lemma op eq z z';                        (** 1. By definition of absorber, zz' should be equal to z.      *)
+    absorber_equal_is_absorber op eq z zz';
+    absorber_lemma op eq zz' y;
     absorber_equal_is_absorber op eq z zz';           (** 2. Any element equal to an absorber is the absorber,         *)
                                                       (**    therefore, zz' is also the absorber, since zz' = z.       *)
     (* assert (is_neutral_of zz' op eq); *)           (** 3. By definition of inverse, zz' is the neutral element.     *)
     (* assert (yzz' `eq` y);             *)           (** 4. By definition of neutral element (zz'), yzz' = y          *)
-                                                      (**    This assertion somehow slows down the prover a lot!       *)
+                                                      (**    This assertion somehow slowed* down the prover a lot!     *)
     (* assert (yzz' `eq` zz');           *)           (** 5. But as zz' is the absorber, yzz' = zz'!                   *)
     absorber_equal_is_absorber op eq zz' yzz';        (** 6. Being equal to the absorber zz', yzz' is the absorber     *)
-    nonabsorber_equal_is_nonabsorber op eq y yzz';    (** 7. But, as an equal of y, yzz' can't be an absorber!         *)
-    assert_spinoff (~(is_absorber_of yzz' op eq));    (**    So, we got the contradiction here!                        *)
-    assert_spinoff (is_absorber_of yzz' op eq);       (**    Deleting the last two asserts gives 10x proof slowdown!   *)
-    ()
-#pop-options 
+    neutral_lemma op eq zz' y;                        (** 7. But, as an equal of y, yzz' can't be an absorber!         *) 
+    nonabsorber_equal_is_nonabsorber op eq y yzz';    (**    So, we got the contradiction here!                        *) 
+//  assert (~(is_absorber_of yzz' op eq)); 
+//  assert (is_absorber_of yzz' op eq);               (**    Deleting the last two asserts gave* 10x proof slowdown!   *)
+// * The slowdowns were noticed BEFORE the introduction of opaques. 
+//   With opaques, most stuff here passes the verification with 0/0/1 resource settings
+    ()    
 
 let group_has_no_absorbers (#a:Type) (g: group #a) (z:a) (y:non_absorber_of g.op g.eq) 
   : Lemma (~(is_absorber_of z g.op g.eq)) = 
@@ -398,56 +456,69 @@ let group_has_no_absorbers (#a:Type) (g: group #a) (z:a) (y:non_absorber_of g.op
 /// until we get to Euclidean Domains, but we shall keep the record field in the base type
 /// because there is no inheritance in F*. Unfortunately so, to say the least.
 
-let nat_function_defined_on_non_absorbers (#a:Type) (op: binary_op a) (eq: equivalence_relation a) = f: (a -> (option nat)){ forall (x:a). (f x)=None ==> is_absorber_of x op eq }
- 
-(*
-let nat_function_value_exists (#a:Type) (op: binary_op a) (eq: equivalence_relation a) (f: nat_function_defined_on_non_absorbers op eq) (x: non_absorber_of op eq) : Lemma (exists (value: nat). (allow_inversion (option nat); value = (Some?.v (f x)))) = allow_inversion (option nat);()
-*)
+let nat_function_defined_on_non_absorbers (#a:Type) (op: binary_op a) (eq: equivalence_relation a) 
+  = f: (a -> (option nat)) { forall (x:a). (f x)=None ==> is_absorber_of x op eq }
 
-let nat_function_value (#a:Type) (op: binary_op a) (eq: equivalence_relation a) (f: nat_function_defined_on_non_absorbers op eq) (x: non_absorber_of op eq) : nat = allow_inversion (option nat); Some?.v (f x)
+let nat_function_value (#a:Type) (op: binary_op a) (eq: equivalence_relation a) (f: nat_function_defined_on_non_absorbers op eq) (x: non_absorber_of op eq) : nat 
+  = allow_inversion (option nat); Some?.v (f x)
 
+[@@"opaque_to_smt"]
 let has_no_absorber_divisors (#a:Type) (op: binary_op a) (eq: equivalence_relation a) = forall (x y: a). is_absorber_of (op x y) op eq <==> (is_absorber_of x op eq) \/ (is_absorber_of y op eq)
 
 let domain_multiplication_law (#a:Type) (eq: equivalence_relation a) (mul: binary_op a{has_no_absorber_divisors mul eq}) (x y: a)
-  : Lemma (~(is_absorber_of x mul eq) /\ ~(is_absorber_of y mul eq) <==> ~ (is_absorber_of (mul x y) mul eq)) = ()
+  : Lemma (~(is_absorber_of x mul eq) /\ ~(is_absorber_of y mul eq) <==> ~ (is_absorber_of (mul x y) mul eq)) =   
+    reveal_opaque (`%has_no_absorber_divisors) (has_no_absorber_divisors #a)
  
 let domain_multiplication_law_inv (#a:Type) (eq: equivalence_relation a) (mul: binary_op a{has_no_absorber_divisors mul eq}) (x y: a)
-  : Lemma ((is_absorber_of x mul eq) \/ (is_absorber_of y mul eq) <==> (is_absorber_of (mul x y) mul eq)) = ()
+  : Lemma ((is_absorber_of x mul eq) \/ (is_absorber_of y mul eq) <==> (is_absorber_of (mul x y) mul eq)) = 
+    reveal_opaque (`%has_no_absorber_divisors) (has_no_absorber_divisors #a) 
   
-let euclidean_norm_property (#a:Type) (eq: equivalence_relation a) (mul: binary_op a{has_no_absorber_divisors mul eq}) (x y: non_absorber_of mul eq) (f: nat_function_defined_on_non_absorbers mul eq) = 
+let euclidean_norm_property (#a:Type) (eq: equivalence_relation a) 
+                                      (mul: binary_op a{has_no_absorber_divisors mul eq}) 
+                                      (x y: non_absorber_of mul eq) 
+                                      (f: nat_function_defined_on_non_absorbers mul eq) = 
   domain_multiplication_law eq mul x y;
   nat_function_value mul eq f (mul x y) >= nat_function_value mul eq f x 
 
-let euclidean_norm_forall_property (#a:Type) (eq: equivalence_relation a) (mul: binary_op a{has_no_absorber_divisors mul eq}) (f: nat_function_defined_on_non_absorbers mul eq)
+[@@"opaque_to_smt"]
+let euclidean_norm_forall_property (#a:Type) (eq: equivalence_relation a) 
+                                   (mul: binary_op a{has_no_absorber_divisors mul eq}) 
+                                   (f: nat_function_defined_on_non_absorbers mul eq)
   = forall (x y: non_absorber_of mul eq). euclidean_norm_property eq mul x y f
 
 type norm_function (#a:Type) (eq: equivalence_relation a) (mul: binary_op a{has_no_absorber_divisors mul eq})
   = f: nat_function_defined_on_non_absorbers mul eq{ forall (x y: non_absorber_of mul eq). euclidean_norm_property eq mul x y f }
 
-#push-options "--ifuel 1 --fuel 0 --z3rlimit 1"
 let euclidean_norm_main_lemma (#a: Type) (eq: equivalence_relation a) (mul: binary_op a{has_no_absorber_divisors mul eq}) (f: norm_function eq mul) (x y: non_absorber_of mul eq)
-  : Lemma (Some?.v (f (mul x y)) >= Some?.v (f x)) = assert (euclidean_norm_property eq mul x y f)
-let test (a:Type) (eq:equivalence_relation a) (mul: binary_op a{has_no_absorber_divisors mul eq}) (f:norm_function eq mul) : Lemma ( 
-  forall (x y: non_absorber_of mul eq). Some?.v (f (mul x y)) >= Some?.v (f x) ) = FStar.Classical.forall_intro_2 (euclidean_norm_main_lemma eq mul f)
-#pop-options
+  : Lemma (Some?.v (reveal_opaque (`%has_no_absorber_divisors) (has_no_absorber_divisors #a); f (mul x y)) >= Some?.v (f x)) =
+  assert (euclidean_norm_property eq mul x y f)
+  
+private let test (a:Type) (eq:equivalence_relation a) (mul: binary_op a{has_no_absorber_divisors mul eq}) (f:norm_function eq mul) : Lemma ( 
+  forall (x y: non_absorber_of mul eq). Some?.v (reveal_opaque (`%has_no_absorber_divisors) (has_no_absorber_divisors #a); f (mul x y)) >= Some?.v (f x) ) = 
+  reveal_opaque (`%has_no_absorber_divisors) (has_no_absorber_divisors #a);
+  FStar.Classical.forall_intro_2 (euclidean_norm_main_lemma eq mul f)
 
-let eq_of (p: magma) = p.eq
+unfold let eq_of (p: magma) = p.eq
 
-//#push-options "--ifuel 4 --fuel 4 --z3rlimit 15"
-
+[@@"opaque_to_smt"]
 let yields_units (#a: Type) (f: a->a) (mul: binary_op a) (eq: equivalence_relation a) = 
   forall (x:a). is_unit (f x) mul eq
 
-let unary_distributivity (#a: Type) (f: a->a) (op: binary_op a) (eq: equivalence_relation a) (x y: a)
+let yields_units_lemma (#a: Type) (mul: binary_op a) (eq: equivalence_relation a) (f: (a->a){yields_units f mul eq}) (x:a)
+  : Lemma (is_unit (f x) mul eq) = reveal_opaque (`%yields_units) (yields_units #a)
+
+let unary_is_distributive_over (#a: Type) (f: a->a) (op: binary_op a) (eq: equivalence_relation a) (x y: a)
  = (f (x `op` y)) `eq` ((f x) `op` (f y))
 
+[@@"opaque_to_smt"]
 let unary_distributes_over (#a: Type) (f: a->a) (op: binary_op a) (eq: equivalence_relation a) = 
-  forall (x y: a). unary_distributivity f op eq x y
+  forall (x y: a). unary_is_distributive_over f op eq x y
 
+[@@"opaque_to_smt"]
 let unary_over_nonzeros_distributes_over (#a: Type) (f: a->a) (op: binary_op a) (eq: equivalence_relation a) = 
-  forall (x y: non_absorber_of op eq). unary_distributivity f op eq x y
+  forall (x y: non_absorber_of op eq). unary_is_distributive_over f op eq x y
 
-let un_distr_l (#a: Type) (op: binary_op a) (eq: equivalence_relation a) (f: (t:(a->a){ unary_over_nonzeros_distributes_over t op eq})) (x y: non_absorber_of op eq)  : Lemma (unary_distributivity f op eq x y) = ()
+let un_distr_l (#a: Type) (op: binary_op a) (eq: equivalence_relation a) (f: (t:(a->a){ unary_over_nonzeros_distributes_over t op eq})) (x y: non_absorber_of op eq)  : Lemma (unary_is_distributive_over f op eq x y) = reveal_opaque (`%unary_over_nonzeros_distributes_over) (unary_over_nonzeros_distributes_over #a) 
 
 type units_of (#a: Type) (mul: binary_op a) (eq: equivalence_relation a) = x:a{is_unit x mul eq}
 
@@ -463,16 +534,20 @@ let un_op_distr_lemma (#a:Type) (mul: binary_op a) (eq: equivalence_wrt mul) (f:
   : Lemma (unary_over_nonzeros_distributes_over f mul eq) = ()
 
 let un_op_distr_lemma_p (#a:Type) (mul: binary_op a) (eq: equivalence_wrt mul) (f: unit_part_function mul eq) (x y: non_absorber_of mul eq)
-  : Lemma (unary_distributivity f mul eq x y) = un_op_distr_lemma mul eq f
+  : Lemma (unary_is_distributive_over f mul eq x y) = reveal_opaque (`%unary_over_nonzeros_distributes_over) (unary_over_nonzeros_distributes_over #a)
 
 let is_unit_normal (#a:Type) (mul: binary_op a) (eq: equivalence_wrt mul) (unit_part_func: a -> a) (x:a) = is_neutral_of (unit_part_func x) mul eq
 
+[@@"opaque_to_smt"]
 let yields_unit_normals (#a:Type) (mul: binary_op a) (eq: equivalence_wrt mul) (unit_part_func: a -> a) (f: a -> a) =
   forall (x:a). is_unit_normal mul eq unit_part_func (f x)
 
-type unit_normals_of (#a: Type) (mul: binary_op a) (eq: equivalence_wrt mul) (unit_part_func: a -> a) = x:a { is_unit_normal mul eq unit_part_func x }
+let yields_unit_normals_lemma (#a:Type) (mul: binary_op a) (eq: equivalence_wrt mul) (unit_part_func: a -> a) (f: (a -> a){yields_unit_normals mul eq unit_part_func f}) (x:a)
+  : Lemma (is_unit_normal mul eq unit_part_func (f x)) = reveal_opaque (`%yields_unit_normals) (yields_unit_normals #a)
 
-let is_normal_part_function (#a:Type) (#mul: binary_op a) (#eq: equivalence_wrt mul) (unit_part_func: a -> a) (f: a -> unit_normals_of mul eq unit_part_func) = 
+type unit_normal_of (#a: Type) (mul: binary_op a) (eq: equivalence_wrt mul) (unit_part_func: a -> a) = x:a { is_unit_normal mul eq unit_part_func x }
+
+let is_normal_part_function (#a:Type) (#mul: binary_op a) (#eq: equivalence_wrt mul) (unit_part_func: a -> a) (f: a -> unit_normal_of mul eq unit_part_func) = 
   is_idempotent f eq /\
   respects_equivalence f eq /\
   yields_unit_normals mul eq unit_part_func f /\
@@ -480,7 +555,7 @@ let is_normal_part_function (#a:Type) (#mul: binary_op a) (#eq: equivalence_wrt 
 
 
 type normal_part_function (#a: Type) (#mul: binary_op a) (#eq: equivalence_wrt mul) (unit_part_func: a -> a)
-  = f:(a -> (unit_normals_of mul eq unit_part_func)){ is_normal_part_function unit_part_func f }
+  = f:(a -> (unit_normal_of mul eq unit_part_func)){ is_normal_part_function unit_part_func f }
 
 let unit_part_func_of_product_is_product_of_unit_parts (#a: Type) (#mul: binary_op a) (#eq: equivalence_wrt mul)
   (unit_part_func: unit_part_function mul eq) (x y: non_absorber_of mul eq) 
@@ -490,70 +565,93 @@ let unit_part_func_of_product_is_product_of_unit_parts (#a: Type) (#mul: binary_
 
 let product_of_unit_normals_is_normal (#a: Type) (#mul: binary_op a) (#eq: equivalence_wrt mul)
   (unit_part_func: unit_part_function mul eq)
-  (x y: unit_normals_of mul eq unit_part_func)
+  (x y: unit_normal_of mul eq unit_part_func)
   : Lemma 
     (requires ~(is_absorber_of x mul eq) /\ ~(is_absorber_of y mul eq))
     (ensures is_unit_normal mul eq unit_part_func (x `mul` y)) =
-  un_op_distr_lemma_p mul eq unit_part_func x y;  
-  neutral_equivalent_is_neutral mul eq (unit_part_func x) (unit_part_func (mul x y)) ;
-  assert ((unit_part_func (x `mul` y)) `eq` ((unit_part_func x) `mul` (unit_part_func y)));
-  assert_spinoff (is_unit_normal mul eq unit_part_func (x `mul` y)) 
+  let up x = unit_part_func x in
+  un_op_distr_lemma_p mul eq unit_part_func x y;                    // up (x*y) = up(x) * up(y) 
+  yields_units_lemma mul eq unit_part_func (x `mul` y);             // up (x*y) is unit
+  neutral_lemma mul eq (unit_part_func x) (unit_part_func y);       // unit part of unit normal is 1
+  neutral_equivalent_is_neutral mul eq (up y) (up x `mul` up y);   
+  neutral_equivalent_is_neutral mul eq (up x `mul` up y) (up (mul x y))
+
 
 type test_unit_part_func (#a: Type) (mul: binary_op a) (eq: equivalence_wrt mul) = unit_part_function mul eq
-
-#push-options "--ifuel 0 --fuel 0 --z3rlimit 4"
+ 
 noeq type ring (#a: Type) = {
   addition: commutative_group #a;
-
-(*
-  multiplication: (t: monoid #a {
-                                  is_fully_distributive t.op addition.op t.eq /\
-                                  (forall (z:a). is_neutral_of z addition.op addition.eq <==> is_absorber_of_magma z t)  
-                                });
-  eq: (t:equivalence_relation a{ equivalence_wrt_condition addition.op t /\ equivalence_wrt_condition multiplication.op t /\ t==addition.eq /\ t==multiplication.eq });  
-*)
- 
   multiplication: (t: monoid #a {is_fully_distributive t.op addition.op t.eq /\ is_absorber_of addition.neutral t.op t.eq });
   eq: (t:equivalence_relation a{ equivalence_wrt_condition addition.op t /\ equivalence_wrt_condition multiplication.op t /\ t===addition.eq /\ t===multiplication.eq });
-
   unit_part_of: a -> units_of multiplication.op eq;
-  normal_part_of: a -> unit_normals_of multiplication.op eq unit_part_of;
+  normal_part_of: a -> unit_normal_of multiplication.op eq unit_part_of;
   euclidean_norm: nat_function_defined_on_non_absorbers multiplication.op eq 
-}
-#pop-options
-
+} 
  
-let neg_of (#a:Type) (r: ring #a) (p:a) : (t:a{ t `r.eq` (r.addition.neutral `r.addition.op` (r.addition.inv p) )}) = r.addition.inv p
+unfold let neg_of (#a:Type) (r: ring #a) (p:a) : (t:a{ t `r.eq` (r.addition.neutral `r.addition.op` (r.addition.inv p) )}) 
+  =  
+  reveal_opaque (`%is_symmetric) (is_symmetric #a) ;
+  inverse_operation_lemma r.addition.op r.eq r.addition.inv p;
+  inverse_lemma_def r.eq r.addition.op r.addition.inv p (r.addition.inv p);
+  neutral_lemma r.addition.op r.eq  r.addition.neutral (r.addition.inv p);
+  r.addition.inv p
 
-let minus_of (#a:Type) (r: ring #a) (x:a) (y:a) : (t:a{ t `r.eq` (x `r.addition.op` (r.addition.inv y) )}) = x `r.addition.op` (neg_of r y)
+unfold let minus_of (#a:Type) (r: ring #a) (x:a) (y:a) : (t:a{ t `r.eq` (x `r.addition.op` (r.addition.inv y) )}) = 
+  reveal_opaque (`%is_reflexive) (is_reflexive #a);
+  x `r.addition.op` (neg_of r y)
 
-#push-options "--ifuel 3 --fuel 0 --z3rlimit 2"
-let minus_minus_x_is_x (#a:Type) (r: ring #a) (x: a) : Lemma (neg_of r (neg_of r x) `r.eq` x /\ x `r.eq` (neg_of r (neg_of r x))) =   
-  let neut_means_zero (p:a) : Lemma (requires is_neutral_of p r.addition.op r.eq) 
-                                    (ensures p `r.eq` r.addition.neutral) 
-                                    [SMTPat(is_neutral_of p r.addition.op r.eq)]
-                                    = neutral_is_unique r.addition.op r.eq r.addition.neutral p in
-  inverse_operation_lemma r.addition.op r.eq r.addition.inv x;
-  inverse_operation_lemma r.addition.op r.eq r.addition.inv (r.addition.inv x); 
+let double_inverse_is_id (#a:Type) (op: binary_op a) (eq: equivalence_wrt op{is_associative op eq}) (inv: inverse_op_for op eq) (x: a) 
+  : Lemma (inv (inv x) `eq` x /\ x `eq` inv (inv x)) =    
+  inverse_operation_lemma op eq inv x;
+  inverse_operation_lemma op eq inv (inv x);   
+  neutral_is_unique op eq (x `op` inv x) (inv (inv x) `op` inv x);
+  group_operation_lemma eq op inv x (inv (inv x)) (inv x);
+  symm_lemma eq (inv (inv x)) x
 
-  assert (r.addition.op x (r.addition.inv x) `r.eq` r.addition.neutral);
-  assert (r.addition.op (r.addition.inv (r.addition.inv x)) (r.addition.inv x) `r.eq` r.addition.neutral);
+let minus_minus_x_is_x (#a:Type) (r: ring #a) (x: a) : Lemma (neg_of r (neg_of r x) `r.eq` x /\ x `r.eq` (neg_of r (neg_of r x)))
+  = double_inverse_is_id r.addition.op r.eq r.addition.inv x  
 
-  trans_lemma r.eq (r.addition.op x (r.addition.inv x)) 
-                    r.addition.neutral 
-                   (r.addition.op (r.addition.inv (r.addition.inv x)) (r.addition.inv x));
+let x_eq_y_means_inv_x_eq_inv_y (#a:Type) (op: binary_op a) (eq: equivalence_wrt op{is_associative op eq}) (inv: inverse_op_for op eq) (x y:a)
+  : Lemma (x `eq` y <==> inv x `eq` inv y) = 
+  if (x `eq` y) then (
+    let x' = inv x in
+    let y' = inv y in
+    inverse_operation_lemma op eq inv y;
+    equivalence_wrt_operation_lemma eq x y x';
+    equivalence_wrt_operation_lemma eq x y y';
+    neutral_equivalent_is_neutral op eq (op y y') (op x y');
+    assert (is_neutral_of (op x y') op eq);
+    producing_neutral_means_inverses eq op inv x y';
+    assert (inv x `eq` inv y)    
+  ) else (
+    if (inv x `eq` inv y) then (
+      let x' = inv x in
+      let y' = inv y in
+      let x'' = (inv (inv x)) in
+      let y'' = (inv (inv y)) in
+      double_inverse_is_id op eq inv x;
+      double_inverse_is_id op eq inv y; 
+      assert (inv x' `eq` x);
+      assert (inv y' `eq` y);
+      inverse_operation_lemma op eq inv y'; 
+      equivalence_wrt_operation_lemma eq x' y' x'';
+      equivalence_wrt_operation_lemma eq x' y' y'';
+      neutral_equivalent_is_neutral op eq (op y' y'') (op x' y'');
+      assert (is_neutral_of (op x' y'') op eq);
+      producing_neutral_means_inverses eq op inv x' y'';
+      trans_lemma_4 eq x x'' y'' y
+    )
+  )
  
-  group_operation_lemma r.eq r.addition.op r.addition.inv 
-            x 
-            (r.addition.inv (r.addition.inv x)) 
-            (r.addition.inv x);  
-  symm_lemma r.eq (r.addition.inv (r.addition.inv x)) x; 
-  ()
- 
-#push-options "--ifuel 2 --fuel 0 --z3rlimit 4"
 let ring_additive_inv_x_is_x_times_minus_one (#a:Type) (r: ring #a) (x: a)
   : Lemma ((r.addition.inv x) `r.eq` (r.multiplication.op x (r.addition.inv r.multiplication.neutral)) /\
            (r.multiplication.op x (r.addition.inv r.multiplication.neutral)) `r.eq` (r.addition.inv x)) = 
+    reveal_opaque (`%is_symmetric) (is_symmetric #a); 
+    reveal_opaque (`%is_transitive) (is_transitive #a); 
+    reveal_opaque (`%equivalence_wrt_condition) (equivalence_wrt_condition #a); 
+    reveal_opaque (`%is_left_distributive) (is_left_distributive #a); 
+    reveal_opaque (`%is_fully_distributive) (is_fully_distributive #a); 
+    reveal_opaque (`%is_inverse_operation_for) (is_inverse_operation_for #a); 
     let eq = r.eq in
     let mul = r.multiplication.op in
     let add = r.addition.op in
@@ -570,10 +668,19 @@ let ring_additive_inv_x_is_x_times_minus_one (#a:Type) (r: ring #a) (x: a)
 //    assert ((mul x (one `add` (inv one))) `eq` ((mul x one) `add` (mul x (inv one)))); 
     symm_lemma eq ((mul x one) `add` (mul x (inv one))) (mul x (one `add` (inv one)));
     //this one speeds up the process if uncommented
-    assert_spinoff (((mul x one) `add` (mul x (inv one))) `eq` (mul x (one `add` (inv one))));    
+//    left_distributivity_lemma mul add eq (mul x one)
+    assert (is_left_distributive mul add eq);
+    left_distributivity_lemma mul add eq x one (inv one);
+    assert (((mul x one) `add` (mul x (inv one))) `eq` (mul x (one `add` (inv one))));    
     //this one requires spinoff!!! for some reason...
+    inverse_operation_lemma add r.eq inv one;
+    assert (is_neutral_of (one `add` inv one) add r.eq);
+    neutral_is_unique add r.eq zero (one `add` inv one);
+    assert (eq (one `add` inv one) zero);
+    absorber_equal_is_absorber mul r.eq zero (one `add` inv one);
+    absorber_lemma mul r.eq (one `add` inv one) x;
     assert_spinoff (mul x (one `add` (inv one)) `eq` zero);       
-    trans_lemma eq ((mul x one) `add` (mul x (inv one))) (mul x (one `add` (inv one))) zero;
+    trans_lemma r.eq ((mul x one) `add` (mul x (inv one))) (mul x (one `add` (inv one))) zero;
     assert (((mul x one) `add` (mul x (inv one))) `eq` zero);
     assert (is_neutral_of zero add eq);
     neutral_equivalent_is_neutral add eq zero ((mul x one) `add` (mul x (inv one)));
@@ -583,85 +690,43 @@ let ring_additive_inv_x_is_x_times_minus_one (#a:Type) (r: ring #a) (x: a)
     assert (is_neutral_of one mul eq);
     neutral_lemma mul eq one x;
     assert (mul x one `eq` x);    
+    x_eq_y_means_inv_x_eq_inv_y add eq inv (mul x one) x;
     assert (inv (mul x one) `eq` (inv x));
-    trans_lemma eq (inv x) (inv (mul x one)) (mul x (inv one));
-  ()
-#pop-options
+    trans_lemma eq (inv x) (inv (mul x one)) (mul x (inv one))
 
 let equal_elements_means_equal_inverses (#a:Type) (r: ring #a) (x y:a) 
-  : Lemma (
-               (r.eq x y == (r.addition.inv x `r.eq` r.addition.inv y)) 
-               /\  
-               (r.eq x y == (r.addition.inv y `r.eq` r.addition.inv x))
-          ) =   
-  let boolean_assertion x y : Lemma (requires x && y) (ensures  x == y) = () in
-  let neut_means_zero (p:a) : Lemma (requires is_neutral_of p r.addition.op r.eq) 
-                                    (ensures p `r.eq` r.addition.neutral) 
-                                    [SMTPat(is_neutral_of p r.addition.op r.eq)]
-                                    = neutral_is_unique r.addition.op r.eq r.addition.neutral p in
-  let one = r.multiplication.neutral in
-  let add = r.addition.op in
-  let mul = r.multiplication.op in
-  let eq = r.eq in
-  let neg = r.addition.inv in 
-  let zero = r.addition.neutral in 
-  if (x `eq` y) then (
-    inverse_operation_lemma add eq neg y; // y + -y = 0
-    inverse_operation_lemma add eq neg x; // x + -x = 0
-    equivalence_wrt_operation_lemma #a #add eq x y (neg y);
-    assert (x `add` neg y `eq` zero);
-    neutral_equivalent_is_neutral add eq zero (x `add` neg y);
-    producing_neutral_means_inverses eq add neg x (neg y);
-    assert_spinoff (neg x `eq` neg y);
-    symm_lemma eq (neg y) (neg x);
-    assert (neg x `eq` neg y);
-    assert (neg x `eq` neg y && (x `eq` y));
-    boolean_assertion (neg x `eq` neg y) (x `eq` y);
-    ()
-  ) else (
-    if ( (neg x) `eq` (neg y) ) then (
-      equivalence_wrt_operation_lemma #a #r.multiplication.op r.eq (neg x) (neg y) (neg one);      
-      assert (r.multiplication.op (neg x) (neg one) `r.eq` r.multiplication.op (neg y) (neg one));      
-      ring_additive_inv_x_is_x_times_minus_one r (neg x);
-      assert (r.eq (neg (neg x)) (r.multiplication.op (neg x) (neg one)));
-      minus_minus_x_is_x r x;
-      trans_lemma eq x (neg (neg x)) (r.multiplication.op (neg x) (neg one));
-
-      assert (x `r.eq` (r.multiplication.op (neg x) (neg one)));
-      assert ((neg x `mul` neg one) `eq` (neg y `mul` neg one));
-      assert ((neg x `mul` neg one) `eq` x);
-      ring_additive_inv_x_is_x_times_minus_one r (neg y);
-      minus_minus_x_is_x r y;
-      trans_lemma eq y (neg (neg y)) (r.multiplication.op (neg y) (neg one)); 
-      assert (eq (neg y `mul` neg one) y);
-      trans_lemma eq x (neg x `mul` neg one) (neg y `mul` neg one);
-      trans_lemma eq x (neg y `mul` neg one) y;
-      ()
-    ) else ()
-  )  
+  : Lemma ((r.eq x y == (r.addition.inv x `r.eq` r.addition.inv y)) /\ (r.eq x y == (r.addition.inv y `r.eq` r.addition.inv x))) =   
+          reveal_opaque (`%is_symmetric) (is_symmetric #a); 
+          reveal_opaque (`%is_reflexive) (is_reflexive #a);     
+          x_eq_y_means_inv_x_eq_inv_y r.addition.op r.eq r.addition.inv x y 
  
 let inv_switch_lemma (#a:Type) (r: ring #a) (x y:a) : Lemma (x `r.eq` (r.addition.inv y) <==> (r.addition.inv x) `r.eq` y) =   
   if (x `r.eq` r.addition.inv y) then (
     equal_elements_means_equal_inverses r x (r.addition.inv y);
     minus_minus_x_is_x r y;
-    trans_lemma r.eq (r.addition.inv x) (r.addition.inv (r.addition.inv y)) y;
-    ()
+    trans_lemma r.eq (r.addition.inv x) (r.addition.inv (r.addition.inv y)) y
   )
   else if (r.addition.inv x `r.eq` y) then (
     equal_elements_means_equal_inverses r (r.addition.inv x) y;
     minus_minus_x_is_x r x;    
-    trans_lemma r.eq x (r.addition.inv (r.addition.inv x)) (r.addition.inv y);
-    ()
-  ) else ()
+    trans_lemma r.eq x (r.addition.inv (r.addition.inv x)) (r.addition.inv y)
+  ) 
 
 let ring_additive_inverse_is_unique (#a:Type) (r:ring #a) (x y: a) 
   : Lemma (requires x `r.eq` y \/ y `r.eq` x) 
           (ensures r.addition.inv x `r.eq` r.addition.inv y /\ r.addition.inv y `r.eq` r.addition.inv x) 
-  = ()
+  = reveal_opaque (`%is_symmetric) (is_symmetric #a);   
+    equal_elements_means_equal_inverses r x y
 
-#push-options "--ifuel 1 --fuel 0 --z3rlimit 1"
+
+/// Make this fully symmetric with the previous lemma, if you want an exercise :)
 let ring_additive_inv_x_is_minus_one_times_x (#a:Type) (r: ring #a) (x: a)
   : Lemma ((r.addition.inv x) `r.eq` (r.multiplication.op (r.addition.inv r.multiplication.neutral) x)) = 
+    reveal_opaque (`%is_symmetric) (is_symmetric #a); 
+    reveal_opaque (`%is_transitive) (is_transitive #a); 
+    reveal_opaque (`%is_right_distributive) (is_right_distributive #a); 
+    reveal_opaque (`%is_fully_distributive) (is_fully_distributive #a); 
+    reveal_opaque (`%is_inverse_operation_for) (is_inverse_operation_for #a); 
     let eq = r.eq in
     let mul = r.multiplication.op in
     let add = r.addition.op in
@@ -672,11 +737,13 @@ let ring_additive_inv_x_is_minus_one_times_x (#a:Type) (r: ring #a) (x: a)
     assert (is_neutral_of (inv one `add` one) add eq);
     neutral_is_unique r.addition.op r.eq zero (inv one `add` one);
     equivalence_wrt_operation_lemma #a #mul eq zero (inv one `add` one) x;
+    absorber_equal_is_absorber mul eq zero (inv one `add` one);
+//    assert (mul (inv one `add` one) x `eq` (mul (inv one) x `add` mul one x));
+//    assert ( (mul (inv one) x `add` mul one x) `eq` (mul (inv one `add` one) x));
+    right_distributivity_lemma mul add eq (inv one) one x;
 //    assert (mul (inv one `add` one) x `eq` (mul (inv one) x `add` mul one x));
     symm_lemma eq (mul (inv one) x `add` mul one x) (mul (inv one `add` one) x);
-//    assert ( (mul (inv one) x `add` mul one x) `eq` (mul (inv one `add` one) x));
-    
-    assert_spinoff (mul (inv one `add` one) x `eq` zero);
+    absorber_lemma mul eq (inv one `add` one) x;        
     trans_lemma eq (mul (inv one) x `add` mul one x) (mul (inv one `add` one) x) zero;
 //  assert ((mul (inv one) x `add` mul one x) `eq` zero);
     neutral_equivalent_is_neutral add eq zero (mul (inv one) x `add` mul one x);
@@ -684,14 +751,15 @@ let ring_additive_inv_x_is_minus_one_times_x (#a:Type) (r: ring #a) (x: a)
 //    assert (inv (mul (inv one) x) `eq` (mul one x));
     inv_switch_lemma r (mul (inv one) x) (mul one x);
 //    assert (mul (inv one) x `eq` (inv (mul one x)));
-    symm_lemma eq (inv (mul one x)) (mul (inv one) x);
+    symm_lemma eq (inv (mul one x)) (mul (inv one) x);    
 //    assert (mul one x `eq` x);
+    neutral_lemma mul eq one x;
     ring_additive_inverse_is_unique r x (mul one x);
 //    assert (inv x `eq` inv (mul one x));
 //    assert (inv (mul one x) `eq` mul (inv one) x);
     trans_lemma eq (inv x) (inv (mul one x)) (mul (inv one) x);    
   ()
-#pop-options
+    
 
 let ring_times_minus_one_is_commutative (#a:Type) (r: ring #a) (x:a) 
   : Lemma ( 
@@ -702,6 +770,8 @@ let ring_times_minus_one_is_commutative (#a:Type) (r: ring #a) (x:a)
             (r.addition.inv r.multiplication.neutral `r.multiplication.op` x) `r.eq` (x `r.multiplication.op` r.addition.inv r.multiplication.neutral) &&
             (r.addition.inv r.multiplication.neutral `r.multiplication.op` x) `r.eq` (r.addition.inv x)
           ) = 
+  reveal_opaque (`%is_symmetric) (is_symmetric #a); 
+  reveal_opaque (`%is_transitive) (is_transitive #a);  
   ring_additive_inv_x_is_minus_one_times_x r x;
   ring_additive_inv_x_is_x_times_minus_one r x
 
@@ -762,6 +832,8 @@ let neg_distr_lemma (#a:Type) (r: ring #a) (x y z: a)
   let neg = r.addition.inv in 
   let zero = r.addition.neutral in
   let one = r.multiplication.neutral in
+  reveal_opaque (`%is_left_distributive) (is_left_distributive #a); 
+  reveal_opaque (`%is_fully_distributive) (is_fully_distributive #a); 
   left_distributivity_lemma mul add eq x y (neg z);
   ring_x_times_minus_y_is_minus_xy r x z;
   assert ((x `mul` neg z) `eq` neg (x `mul` z)); 
@@ -775,52 +847,47 @@ let neut_lemma (#a: Type) (r: ring #a) : Lemma (is_neutral_of r.multiplication.n
 let add_eq_of (#a:Type) (r: ring #a) : equivalence_wrt r.addition.op = r.eq
 
 let mul_neutral_lemma (#a: Type) (r: ring #a) (x: a{is_neutral_of x r.multiplication.op r.eq})
-  : Lemma (r.eq x r.multiplication.neutral) = ()
+  : Lemma (r.eq x r.multiplication.neutral) =
+  reveal_opaque (`%is_symmetric) (is_symmetric #a);   
+  neutral_is_unique r.multiplication.op r.eq r.multiplication.neutral x
 
-let is_zero_of (#a: Type) (r: ring #a) (x: a) = is_absorber_of x r.multiplication.op r.eq
+unfold let is_zero_of (#a: Type) (r: ring #a) (x: a) = is_absorber_of x r.multiplication.op r.eq
 
 let two_zeros_are_equal (#a:Type) (r: ring #a) (x y: (t:a{r.eq t r.addition.neutral})) 
-  : Lemma (x `r.eq` y) = ()
+  : Lemma (x `r.eq` y) =  
+  neutral_equivalent_is_neutral r.addition.op r.eq r.addition.neutral x; 
+  neutral_equivalent_is_neutral r.addition.op r.eq r.addition.neutral y;
+  neutral_is_unique r.addition.op r.eq x y
 
-let eq_symmetry (#a:Type) (eq: equivalence_relation a) (x y: a) : Lemma (requires (x `eq` y \/ y `eq` x)) (ensures (x `eq` y /\ y `eq` x)) = ()
-
-#push-options "--ifuel 1 --fuel 0 --z3rlimit 2"
+let eq_symmetry (#a:Type) (eq: equivalence_relation a) (x y: a) 
+  : Lemma (requires (x `eq` y \/ y `eq` x)) (ensures (x `eq` y /\ y `eq` x)) = reveal_opaque (`%is_symmetric) (is_symmetric #a)
+ 
 let zero_is_equal_to_add_neutral_p (#a:Type) (r: ring #a) (z: a)
-  : Lemma (is_zero_of r z <==> r.eq z r.addition.neutral) 
-  =  
-  let eq = r.eq in
-  assert (is_absorber_of r.addition.neutral r.multiplication.op r.eq);
-  if (r.eq z r.addition.neutral) then 
-    absorber_equal_is_absorber r.multiplication.op r.eq r.addition.neutral z  
-  else (
-    FStar.Classical.move_requires_2 (absorber_is_unique r.multiplication.op r.eq) z r.addition.neutral;
-    assert_spinoff (is_absorber_of z r.multiplication.op r.eq <==> eq z r.addition.neutral) 
-  )
-#pop-options
-
+  : Lemma (is_zero_of r z <==> r.eq z r.addition.neutral) = 
+  if (r.eq z r.addition.neutral) 
+  then absorber_equal_is_absorber r.multiplication.op r.eq r.addition.neutral z  
+  else FStar.Classical.move_requires_2 (absorber_is_unique r.multiplication.op r.eq) z r.addition.neutral  
+   
 let zero_is_equal_to_add_neutral (#a:Type) (r: ring #a) : Lemma (forall (x:a). is_zero_of r x <==> r.eq x r.addition.neutral) 
   = FStar.Classical.forall_intro (zero_is_equal_to_add_neutral_p r)
 
-let nonzero_is_equal_to_add_neutral (#a:Type) (r: ring #a) 
+let nonzero_is_not_equal_to_add_neutral (#a:Type) (r: ring #a) 
   : Lemma (forall (x:a). ~(is_zero_of r x) <==> ~(r.eq x r.addition.neutral)) = zero_is_equal_to_add_neutral r
  
 let nonzero_is_not_equal_to_add_neutral_p (#a:Type) (r: ring #a) (z: a)
   : Lemma (~(is_absorber_of z r.multiplication.op r.eq) <==> ~(r.eq z r.addition.neutral)) = zero_is_equal_to_add_neutral r
 
-
 type domain (#a: Type) = r:ring #a { has_no_absorber_divisors r.multiplication.op r.eq }
 
- 
-#push-options "--ifuel 1 --fuel 0 --z3rlimit 2"
 let domain_mul_absorber_lemma (#a:Type) (dom: domain #a) (x y:a) 
   : Lemma (is_absorber_of (dom.multiplication.op x y) dom.multiplication.op dom.eq <==> 
            is_absorber_of x dom.multiplication.op dom.eq \/ is_absorber_of y dom.multiplication.op dom.eq) = 
    domain_multiplication_law_inv dom.eq dom.multiplication.op x y
-#pop-options
 
-
-private let domain_lemma_1 (#a:Type) (dom: domain #a) (p q:a) : Lemma (requires is_absorber_of p dom.multiplication.op dom.eq \/ is_absorber_of p dom.multiplication.op dom.eq)
-                                                              (ensures is_absorber_of (dom.multiplication.op p q) dom.multiplication.op dom.eq) = ()
+private let domain_lemma_1 (#a:Type) (dom: domain #a) (p q:a) 
+  : Lemma (requires is_absorber_of p dom.multiplication.op dom.eq \/ is_absorber_of p dom.multiplication.op dom.eq)
+          (ensures is_absorber_of (dom.multiplication.op p q) dom.multiplication.op dom.eq) = 
+  reveal_opaque (`%has_no_absorber_divisors) (has_no_absorber_divisors #a) 
                                                
 private let domain_lemma_2 (#a:Type) (dom: domain #a) (x y:a) 
   : Lemma (requires is_absorber_of (dom.multiplication.op x y) dom.multiplication.op dom.eq) 
@@ -834,40 +901,27 @@ let domain_zero_product_means_zero_factor (#a:Type) (dom: domain #a) (p q: a)
   absorber_equal_is_absorber dom.multiplication.op dom.eq dom.addition.neutral (p `dom.multiplication.op` q); 
   domain_multiplication_law_inv dom.eq dom.multiplication.op p q;
   zero_is_equal_to_add_neutral dom
-
-#push-options "--ifuel 1 --fuel 0 --z3rlimit 1"
+ 
 let domain_characterizing_lemma (#a:Type) (dom: domain #a) (p q: a) 
   : Lemma ((p `dom.multiplication.op` q) `dom.eq` dom.addition.neutral <==>
-           (p `dom.eq` dom.addition.neutral \/ q `dom.eq` dom.addition.neutral)) =     
+           (p `dom.eq` dom.addition.neutral \/ q `dom.eq` dom.addition.neutral)) =   
+  reveal_opaque (`%is_transitive) (is_transitive #a);     
   FStar.Classical.move_requires_2 (domain_zero_product_means_zero_factor dom) p q;
   if (dom.eq p dom.addition.neutral) then (
     absorber_equal_is_absorber dom.multiplication.op dom.eq dom.addition.neutral p;
     absorber_lemma dom.multiplication.op dom.eq p q;
-    assert (p `dom.multiplication.op` q `dom.eq` dom.addition.neutral);
-    ()
+    assert (p `dom.multiplication.op` q `dom.eq` dom.addition.neutral)
   ) else if (dom.eq q dom.addition.neutral) then (
     absorber_equal_is_absorber dom.multiplication.op dom.eq dom.addition.neutral q;
     absorber_lemma dom.multiplication.op dom.eq q p;
-    assert (p `dom.multiplication.op` q `dom.eq` dom.addition.neutral);
-    ()
-  ) else ()
-#pop-options
-
-
-private let aux_lemma (#a:Type) (d: domain #a) (p q r: a) : Lemma (requires p `d.eq` d.addition.neutral \/ (d.addition.op q (d.addition.inv r) `d.eq` d.addition.neutral))
-  (ensures p `d.eq` d.addition.neutral \/ q `d.eq` r) = 
-  if (p `d.eq` d.addition.neutral) then () else (
-   if (d.addition.op q (d.addition.inv r) `d.eq` d.addition.neutral) then (
-     group_element_equality_means_zero_difference d.addition q r;
-
-     ()
-   ) else ()
-  )
+    assert (p `dom.multiplication.op` q `dom.eq` dom.addition.neutral)
+  )  
   
-#push-options "--ifuel 1 --fuel 0 --z3rlimit 10"
 private let domain_law_from_pq_eq_pr (#a:Type) (d: domain #a) (p q r: a)
   : Lemma (requires d.multiplication.op p q `d.eq` d.multiplication.op p r) 
-          (ensures p `d.eq` d.addition.neutral \/ (q `d.addition.op` (d.addition.inv r) `d.eq` d.addition.neutral)) = 
+          (ensures p `d.eq` d.addition.neutral \/ (q `d.eq` r)) =  
+  reveal_opaque (`%is_transitive) (is_transitive #a);     
+  reveal_opaque (`%is_symmetric) (is_symmetric #a);     
   let mul = d.multiplication.op in
   let eq = d.eq in
   let add = d.addition.op in
@@ -887,41 +941,27 @@ private let domain_law_from_pq_eq_pr (#a:Type) (d: domain #a) (p q r: a)
   assert (eq zero ((p `mul` q) `add` (neg (p `mul` r))));  
   trans_lemma_4 eq zero ((p `mul` q) `add` (neg (p `mul` r))) (mul p q `add` mul p (neg r)) (mul p (add q (neg r)));
   domain_characterizing_lemma d p (add q (neg r));
- // assert (p `eq` zero \/ (q `add` neg r `eq` zero));
- // aux_lemma d p q r;
-//  assert (d.eq p d.addition.neutral \/ d.eq q r);  
-//  let sq = squash (p `d.eq` d.addition.neutral \/ (q `d.eq` r)) in
-//  assert (eq p zero \/ eq q r);
- // admit();
-  () 
-#pop-options
- 
-#push-options "--ifuel 1 --fuel 0 --z3rlimit 15"
-let domain_law_from_pq_eq_pr_full (#a:Type) (d: domain #a) (p q r: a)
-  : Lemma (requires d.multiplication.op p q `d.eq` d.multiplication.op p r) 
-          (ensures p `d.eq` d.addition.neutral \/ (q `d.eq` r)) = 
-  domain_law_from_pq_eq_pr d p q r;
-  aux_lemma d p q r
-#pop-options
+   if (p `d.eq` d.addition.neutral) then () else (
+   if (d.addition.op q (d.addition.inv r) `d.eq` d.addition.neutral) then (
+     group_element_equality_means_zero_difference d.addition q r;
 
+     ()
+   ) else ()
+  )
+ 
+  
 type commutative_ring (#a: Type) = r:ring #a { is_commutative r.multiplication.op r.eq }
 
 /// I'm not 100% sure, but somehow I think that PERHAPS unit/normal part functions
-/// are safe to expect to be defined over any integral domain. Still, for safety sake,
-/// I restricted all that to euclidean domains.
-///
-/// When I lift that restriction, the fraction library will of course move from
-/// using euclidean domains to using arbitrary integral domains.
-///
-/// The special case of euclidean domains, which allows for reduced fractions, will be handled
-/// differently, and all arithmetics will also account for the gcd/eea availability.
+/// are safe to expect to be defined over any integral domain. 
 /// 
+/// The special case of euclidean domains, which allows for reduced fractions, will later be handled
+/// differently, and all arithmetics will also account for the gcd/eea availability.
 type integral_domain (#a: Type) = r:domain #a 
 { 
   is_commutative r.multiplication.op r.eq /\
   is_unit_part_function r.unit_part_of /\
-  is_normal_part_function r.unit_part_of r.normal_part_of  
-  
+  is_normal_part_function r.unit_part_of r.normal_part_of    
 }
 
 type euclidean_domain (#a:Type) = r:integral_domain #a 
